---
title: "COS4892 Assignment 2 - 547106"
author: "Christopher Deon Steenkamp - 36398934"
output: pdf_document
geometry: margin=1in
header-includes:
  - \usepackage{amsmath}
---
## Question 1

### 1.1

### 1.2

### 1.3

### 1.4

## Question 2

### 2.1

The program statement is a sequential composition of the form $\{P\} S1;S2;S3 \{Q\}$

We are given that
$\{Q\}$: $\{i = j\}$
$S1$: $i:=1+1$
$S2$: $k:=k*2$
$S3$: $j:=j-1$

Working backwards from the postcondition $\{i = j\}$, we apply the assignment axiom to $S3$ by replacing $j$ with $j-1$. From this we get the intermediate assertion $R$: $\{i=j-1\}$.

Using $R$ as the postconditon of $S2$, we again work backwards and apply the assignment axiom to $S2$. The variable assignment to $k$ has no effect on our postcondition so the assertion $R$ is invariant over $S2$.

We then use $R$: $\{i=j-1\}$ as the postcondition of $S1$, and applying the assignment axiom by replacing $i$ with $i + 1$ gives us the assertion $P$: $\{i+1=j-1\}$, which is the precondition for the program statement.

### 2.2

I think there is an error in the question because incrementing x after you have multiplied y by x will cause the loop invariant to fail ($y \ne x!$). For my solution I have swapped the order of the two assignment statements (and provided verification of the correctness of the updated program).

The corrected program statement in guarded command form is thus:

$\{n = 4\}$\
$x,y:=0,1$\;\
$\{$Invariant: $0\le x\le n \land y = x!$\
Bound function: $n - x\}$\
do $x< n\longrightarrow$ $x := x + 1$; $y := y * x$\
od\
$\{x=4\land y=n!\}$

$\neg done$ is defined as $x < n$, so the loop body runs when $x < n$.

To verify the termination condtion we show that the conjunction of the invariant and $done$ implies the postcondition. So $x \ge n \land 0\le x\le n \land y = x!$. Also, $x \ge 0 \land x \le n$ together imply that $x=n$ so we have that the loop terminates correctly.

To verify initialization assignments, we show that the loop invariant is a postcondition of assignment. We use the assignment axiom and the initial assignment values to show that:

$n\ge 0 \equiv 0 \le 0 \le n \land 1 = 0!$

We then check the loop body using $P = \{invariant \land \neg done \land bf\}$, working backwards from the post-condition using the assignment axiom. Note that we do two verfications because there are two sequential statements.

1. $\{Q\} \Rightarrow \{R\}$ where $R = Q[y:=y*x]$\
$\{0\le x\le n \land y * x = x! \land x < n \land n-x < C\}$
1. $\{R\}\Rightarrow \{R2\}$ where $R2 = R[x:=x+1]$\
   $\{0\le x + 1\le n \land y * (x+1) = (x+1) * x! \land n-(x + 1) < C\}$

Which satisfies the final condition, with $n = 4, x = 4, y = n! = 24$

### 2.3

The given program statement in guarded-command format is as follows:

$\{P\}$\
if $even(x) \longrightarrow \{P\land even(x)\}$ $x:=x-1$ $\{x \ge0\land z+y*x=a*b\}$\
$\small{\square}\space$ $odd(x)\longrightarrow\{P\land odd(x)\}$ $z:=z+yx$ $\{x \ge0\land z+y*x=a*b\}$\
fi\
$\{x \ge0\land z+y*x=a*b\}$

We also note that $[P\Rightarrow even(x)\lor odd(x)]$

Taking the first statement from the conditional, (if $even(x)$), and applying the assignment axiom, we get the following precondition:

$\{x-1\ge0 \land z+y(x-1)=a*b\land even(x)\}$

Applying the assignment axiom to the second statement of the conditional gives us the following precondition:

$\{x\ge0 \land (z+ yx) + yx =a*b\land odd(x)\}$

Combining the two preconditions we get $\{P\}$ = $\{x \ge 1 \land z+yx-y=a*b \land z+2yx=a*b\}$

### 2.4

$\{P\}$
do $0 \ge x \ge -2 \longrightarrow x := x - 1$
od
$\{x = -3\}$

Starting with the postcondition $Q$, we iteratively use the assignment axiom until we get to the point that the loop is out of bounds.

1. $Q[x := x - 1]$ gives us $x - 1 = - 3$ so $R1 = \{x = -2\}$
2. $R1[x := x - 1]$ gives us $x - 1 = -2$ so $R2 = \{x = -1\}$
3. $R2[x := x - 1]$ gives us $x - 1 = -1$ so $R3 = \{x = 0\}$
4. $R3[x := x - 1]$ gives us $x - 1 = 0$ so $R4 = \{x = 1\}$ which is out of bounds so the last valid state was $R3$.

This gives us that the precondition $P$ is $\{x=0\}$

## Question 3

To verify a Hoare triple $\{P\}S\{Q\}$ we need to show that, given a precondition $P$, after executing some statement $S$, we have the postcondition $Q$. To this, we make use of the assignment axiom. The axiom is applied by working backwards from the postcondition, using the fact that, given a postcondition $Q$ which is the state after execution of a statement $S$, we can "create" a precondition $R$ by replacing all occurrences of variables in $Q$ with their respective assignments from $S$.

For example, given the postcondition $Q$ = $\{x = 2\}$ and the assignment statement $S$ = $x := x *2$ we can create a precondition $R$ such that $R$ = $Q[x := x * 2]$ which means that we replace occurrences of $x$ in $Q$ with $x * 2$. This gives us $R$ = $\{x * 2 = 2\}$, which we simplify using arithmetic to $\{x = 1\}$.

Clearly, by starting at $R$, with $x = 1$, after setting $x := x * 2$ $(x:=1*2)$, we have $Q$, $\{x = 2\}$.

From here, if $P$ and $R$ can be shown equivalent, then we have verified the Hoare triple $\{P\}S\{Q\}$.

## Question 4

### 4.1

$\{x = y\}$\
if $\space\space x = 0 \longrightarrow \{x = y \land x = 0\} x := y + 1 \{(x = y + 1) \lor (z = x + 1)\}$\
$\small{\square}$ $\space x \ne 0 \longrightarrow \{x = y \land x \ne 0\} z := y +1 \{(x = y + 1) \lor (z = x + 1)\}$\
fi\
$\{(x = y + 1) \lor (z = x + 1)\}$

We have that either $x = 0$ or $x\ne 0$ so we can verify correctness of the program by verifying the correctness of each statement.

We start by using the assignment axiom on the postcondition $\{(x = y + 1) \lor (z = x + 1)\}$ using the statement $x := y + 1$.

This gives us $\{(y + 1 = y + 1) \lor (z = (y + 1) + 1)\}$ (which is $true$ by propositional calculus) so we have that:

$\{(y + 1 = y + 1) \lor (z = (y + 1) + 1)\}$\
=$\space$ {replace equals for equals, $true\equiv p\equiv p$, with $p=y+1$}\
$\{(true) \lor (z = (y+1)+1)\}$\
=$\space$ {$true$ is a zero of disjunction}\
$true$

So we have $x = y \land x = 0 \equiv true$.

Applying the assignment axiom on the postcondition $\{(x = y + 1) \lor (z = x + 1)\}$ using the statement $z := y +1$ yields:

$\{(x = y + 1) \lor (y + 1 = x + 1)\}$\
=$\space$ {we have that x = y from P, replacing equals for equals}\
$\{(y = y + 1) \lor (y + 1 = y + 1)\}$\
=$\space$ {replace equals for equals, $true\equiv p\equiv p$, with $p=y+1$}\
$\{(y = y + 1) \lor (true)\}$\
=$\space$ {$true$ is a zero of disjunction}\
$true$

So we have $\{x = y \land x \ne 0\} \equiv true$

This proves that the program correctly arrives at the postcondition from the given precondition.

### 4.2

$\{x = y\}$\
if $\space\space x = 0 \longrightarrow \{x = y \land x = 0\} x := y + 1 \{(z = 1) \to(x = 1)\}$\
$\small{\square}$ $\space x \ne 0 \longrightarrow \{x = y \land x \ne 0\} z := y +1 \{(z = 1) \to (x = 1)\}$\
fi\
$\{(z = 1) \to (x = 1)\}$

As is the case in q4.1, we have that either $x = 0$ or $x\ne 0$ so we can verify correctness of the program by verifying the correctness of each statement.

We start by using the assignment axiom on the postcondition $\{(z = 1) \to (x = 1)\}$ using the statement $x := y + 1$.

This gives us $\{(z = 1) \to (y + 1 = 1)\}$\
=$\space$ {arithmetic}\
$\{(z = 1) \to (y = 0)\}$\
=$\space$ {assume $x = y = 0$, definition of only-if, with $p=(z=1)$ and $q =(y=0)$, $p \Rightarrow q \equiv q \equiv p\lor q$}\
$\{(z = 1) \lor (y = 0)\}$\
=$\space$ {$x = y, x = 0$, equals for equals}\
$\{(z = 1) \lor (true)\}$\
=$\space$ {$true$ is a zero of disjunction}\
$true$

So we have $x = y \land x = 0 \equiv true$.

Applying the assignment axiom on the postcondition $\{(z = 1) \to (x = 1)\}$ using the statement $z := y +1$ yields:

$\{(y + 1 = 1) \to (x = 1)\}$\
=$\space$ {arithmetic}\
$\{(y = 0) \to (x = 1)\}$\
=$\space$ {Logical equivalence $p\Rightarrow q\equiv \neg p\lor q$}\
$\{(y \ne 0) \lor (x = 1)\}$\
=$\space$ {$x = y, x \ne 0$, equals for equals}\
$\{(true) \lor (x = 1)\}$\
=$\space$ {$true$ is a zero of disjunction}\
$true$

So we have $\{x = y \land x \ne 0\} \equiv true$

This proves that the program correctly arrives at the postcondition from the given precondition.

### 4.3

$\{3 \le |x| \le 4\}$\
if $\space\space x < 0 \longrightarrow \{3 \le |x| \le 4 \land x < 0\} y := -x \{2 \le y \le 4\}$\
$\small{\square}$ $\space x \ge 0 \longrightarrow \{3 \le |x| \le 4 \land x \ge 0\} y := x \{2 \le y \le 4\}$\
fi\
$\{2 \le y \le 4\}$

We have that either $x < 0$ or $x \ge 0$ so we can verify correctness of the program by verifying the correctness of each statement.

We start by using the assignment axiom on the postcondition $\{2 \le y \le 4\}$ using the statement $y := -x$.

This gives us $\{2 \le -x \le 4\}$\
=$\space$ {we have that $x < 0$ so we know that -x is positive}\
$\{2 \le x \le 4\}$\
=$\space$ {equals for equals and arithmetic $x = |x|$}\
$\{2 \le |x| \le 4\}$\
=$\space$ {Given that $3 \le |x| \le 4$}\
$\{2 \le 3 \le |x| \le 4\}$\
=$\space$ {arithmetic}\
$\{3 \le |x| \le 4\}$

So we have $3 \le |x| \le 4$ as required.

Applying the assignment axiom on the postcondition $\{2 \le y \le 4\}$ using the statement $y:=x$ yields:

$\{2 \le x \le 4\}$\
=$\space$ {we have that $x \ge 0$ so we know that x is positive, so equals for equals and arithmetic $x = |x|$}\
$\{2 \le |x| \le 4\}$\
=$\space$ {Given that $3 \le |x| \le 4$}\
$\{2 \le 3 \le |x| \le 4\}$\
=$\space$ {arithmetic}\
$\{3 \le |x| \le 4\}$

So we have $3 \le |x| \le 4$ as required.

This proves that the program correctly arrives at the postcondition from the given precondition.

## Question 5

The two required steps for proving some property $P$ over natural numbers $n$ using simple induction are the basis step and the inductive step.

The basis step invoves showing that $P$ is $true$ for $n=0$, i.e. $P(0)$. Then, the inductive step is used to show that $P(n+1)$ follows from the assumption that $P(n)$ is true (where $P(n)$ is known as the inductive hypothesis).

Thus, from $P(0)$ it can be shown that $P(1)$, then from $P(1)$, you can prove $P(2)$, ... $P(n) \rightarrow P(n+1)$.

## Question 6

We have the following assertions.

$P = \{n\in Z\land 0\le n\}$\
$bf = \{n - k\}$\
$Q = \{n\in Z\land k\in Z\land 1\le k\le n+1\land \space_{i=1}^{k-1}A(i)\ne x\land ((k\le n\land A(k)=x)\lor k = n + 1)\}$\
$\neg done=\{k \le n \land A(k) \ne x\}$\
$inv=\{n\in Z \land k\in Z\land 1\le k\le n + 1 \land \space_{i=1}^{k-1}A(i)\ne x\}$

1. We are given the loop invariant $inv$.
1. Show that $\{P\}k:=1\{inv\}$\
\
Using the assignment axiom of the initialization step on the invariant, $inv[k:=1]$, gives:\
\
$\{n\in Z \land 1\in Z\land 1\le 1\le n + 1 \land \space_{i=1}^{1-1}A(i)\ne x\}$\
=$\space$ {arithmetic, 1 is an integer}\
$\{n\in Z \land true \land 0\le n \land \space_{i=1}^{0}A(i)\ne x\}$\
=$\space$ {iteration over empty range with $true$ as the unit of conjunction}\
$\{n\in Z \land true \land 0\le n \land true\}$\
\
So we have $\{n\in Z\land 0\le n\} \equiv P$ as required.
1. Show that $\{inv\land \neg done\}k:=k+1\{inv\}$\
\
Using the assignment axiom of the loop body on the conjunction of the invariant and the termination condition, $inv[k:=k+1] \land \neg done[k:=k+1]$, gives:\
\
$\{n\in Z \land k+1\in Z\land 1\le k+1\le n + 1 \land \space_{i=1}^{k+1-1}A(i)\ne x \land k+1 \le n \land A(k+1) \ne x\}$\
=$\space$ {arithmetic, 1 is an integer,if $k+1$ is an integer, then $k$ must also be an integer}\
$\{n\in Z \land k\in Z\land 1\le k+1\le n + 1 \land \space_{i=1}^{k}A(i)\ne x \land k+1 \le n \land A(k+1) \ne x\}$\
=$\space$ {arithmetic, $k+1 \le n \le n + 1$ implies $k+1 \le n$}\
$\{n\in Z \land k\in Z\land 1\le k+1 \le n \land \space_{i=1}^{k}A(i)\ne x  \land A(k+1) \ne x\}$\
=$\space$ {One-point rule with $e=k+1$}\
$\{n\in Z \land k\in Z\land 1\le k+1 \le n \land \space_{i=1}^{k}A(i)\ne x  \land \space_{i=k+1}^{k+1}A(i) \ne x\}$\
=$\space$ {splitting on range $1\le i \le k$ and $k+1\le i\le k+1$}\
$\{n\in Z \land k\in Z\land 1\le k+1 \le n \land \space_{i=1}^{k+1}A(i)\ne x\}$\
\
Thus we have $inv\equiv \{n\in Z \land k\in Z\land 1\le k+1 \le n \land \space_{i=1}^{k+1}A(i)\ne x\}$.
1. Show that $[inv \land done \Rightarrow Q]$\
\
$done\equiv \neg\neg done\equiv \{k >n \lor A(k) = x\}$\
There are two conditions which can terminate the loop, we investigate both separately.\
With $done=\{k>n\}$ we have:\
\
$\{n\in Z \land k\in Z\land 1\le k\le n + 1 \land \space_{i=1}^{k-1}A(i)\ne x \land k >n\}$\
= {Together, $k >n$ and $k\le n + 1$ imply $k = n + 1$}\
$\{n\in Z \land k\in Z\land 1\le k\le n + 1 \land \space_{i=1}^{k-1}A(i)\ne x \land k = n + 1\}$\
$\Rightarrow$\
$Q$\
\
For the second case, with $done=\{A(k) = x\}$ we have:\
\
$\{n\in Z \land k\in Z\land 1\le k\le n + 1 \land \space_{i=1}^{k-1}A(i)\ne x \land A(k) = x\}$\
= {We know that $k\ne n + 1$, so with $k\le n+1$ we know that $k\le n$}\
$\{n\in Z \land k\in Z\land 1\le k\le n + 1 \land \space_{i=1}^{k-1}A(i)\ne x \land k\le n\land A(k) = x\}$\
$\Rightarrow$\
$Q$
1. We have $bf$ defined as $n - k$. The loop body executes while $k \le n$, with $k$ incremented each iteration by the statement $k :=k+1$. As $k$ approaches $n$, $bf$ approaches $0$. This means that the loop will complete in at most $n$ iterations.

## Question 7

Program statement:

$\{0\le n\}$\
$k,c:=0,0$;\
do $k<n \land A(k) = 0\longrightarrow k,c:=k+1,c+1$\
$\small\square$ $k<n \land A(k) \ne 0\longrightarrow k:=k+1$\
od\
$\{c = \langle\Sigma i: 0\le i< n\land A(i)= 0 : 1\rangle\}$

Assertions:

$P = \{0\le n\}$\
$bf = \{n - k\}$\
$Q = \{c = \langle\Sigma i: 0\le i< n\land A(i)= 0 : 1\rangle\}$\
$\neg done=\{k < n\}$

Verification of correctness:

1. The loop invariant is identified as $inv = \{0\le k\le n\land c = \langle\Sigma i: 0\le i< k\land A(i)= 0 : 1\rangle\}$
1. Show that $\{P\}k,c:=0,0\{inv\}$\
\
Using the assignment axiom of the initialization step on the invariant, $inv[k,c:=0,0]$, gives:\
\
$\{0\le 0\le n\land 0 = \langle\Sigma i: 0\le i< 0\land A(i)= 0 : 1\rangle\}$\
=$\space$ {iteration over empty range with $0$ as the unit of summation}\
$\{0\le n\land 0 = 0\}$\
=$\space$ {reflexivity of equality, true is the unit of conjunction}\
$0\le n$\
\
So we have $P\Rightarrow inv$ as required.
1. For each statement $S$ in the loop body, show that $\{inv\land \neg done\}S\{inv\}$
\
For the case where $A(k) = 0$, using the assignment axiom of the loop body on the conjunction of the invariant and the termination condition, $inv[k,c:=k+1,c+1] \land \neg done[k,c:=k+1,c+1]$, gives:\
\
$\{0\le k+1\le n\land c+1 = \langle\Sigma i: 0\le i< k+1\land A(i)= 0 : 1\rangle\land k+1<n\}$\
=$\space$ {arithmetic}\
$\{0\le k\le n\land c+1 = \langle\Sigma i: 0\le i< k+1\land A(i)= 0 : 1\rangle\}$\
=$\space$ {splitting over range and one-point rule}\
$\{0\le k\le n\land c +1 = \langle\Sigma i: 0\le i< k\land A(i)= 0 : 1\rangle + \langle\Sigma i: k\le i< k+1\land A(i)= 0 : 1\rangle\}$\
=$\space$ {$A(k) = 0$ from loop branch, so the split out summation is 1}\
$\{0\le k\le n\land c + 1 = \langle\Sigma i: 0\le i< k\land A(i)= 0 : 1\rangle + 1\}$\
=$\space$ {arithmetic}\
$\{0\le k\le n\land c = \langle\Sigma i: 0\le i< k\land A(i)= 0 : 1\rangle\}$\
$\equiv$ $inv$\
\
For the case where $A(k) \ne 0$, using the assignment axiom of the loop body on the conjunction of the invariant and the termination condition, $inv[k:=k+1] \land \neg done[k=k+1]$, gives:\
\
$\{0\le k+1\le n\land c = \langle\Sigma i: 0\le i< k+1\land A(i)= 0 : 1\rangle\land k+1<n\}$\
=$\space$ {arithmetic}\
$\{0\le k\le n\land c = \langle\Sigma i: 0\le i< k+1\land A(i)= 0 : 1\rangle\}$\
=$\space$ {splitting over range and one-point rule}\
$\{0\le k\le n\land c = \langle\Sigma i: 0\le i< k\land A(i)= 0 : 1\rangle + \langle\Sigma i: k\le i< k+1\land A(i)= 0 : 1\rangle\}$\
=$\space$ {$A(k) \ne 0$ from loop branch, 0 is the unit of summation over empty range}\
$\{0\le k\le n\land c = \langle\Sigma i: 0\le i< k\land A(i)= 0 : 1\rangle + 0\}$\
$\equiv$ $inv$
1. Show that $[inv \land done \Rightarrow Q]$\
\
$done\equiv \neg\neg done\equiv \{k\ge n\}$\
\
$\{0\le k\le n\land c = \langle\Sigma i: 0\le i< k\land A(i)= 0 : 1\rangle\land k\ge n\}$\
= {Together, $k\ge n$ and $k\le n$ imply $k = n$}\
$\{c = \langle\Sigma i: 0\le i< n\land A(i)= 0 : 1\rangle\}$\
$\Rightarrow$\
$Q$
1. We have $bf$ defined as $n - k$. The loop body executes while $k < n$, with $k$ incremented each iteration by the statement $k :=k+1$. As $k$ approaches $n$, $bf$ approaches $0$. This means that the loop will complete in at most $n$ iterations.

## Question 8

We will prove by simple induction that $P\equiv \langle \Sigma k: 0\le k < n:2^k \rangle = 2^{n}-1$ for all $n\in N$

We start by showing $P(0)$:

$P(0)$\
= {definition}\
$\langle \Sigma k: 0\le k < 0:2^k \rangle = 2^{0}-1$\
= {0 is the unit of summation over the empty range}\
$0 = 2^{0}-1$\
= {arithmetic}\
$0 = 0$\
= {reflexivity of equality}\
$true$

We now show via the induction step that $P(n+1)$:

$P(n+1)$\
= {definition}\
$\langle \Sigma k: 0\le k < n+1:2^k \rangle = 2^{n+1}-1$\
= {split out the last element of the summation}\
$\langle \Sigma k: 0\le k < n:2^k \rangle + 2^n = 2^{n+1}-1$\
= {assume $P(n)$ (induction hypothesis)}\
$(2^n-1) + 2^n = 2^{n+1}-1$\
= {arithmetic}\
$(2^n-1) + 2^n = (2^{n}*2)-1$\
= {arithmetic}\
$2(2^n) - 1 = (2^{n}*2)-1$\
= {arithmetic}\
$true$

Therefore, by the principle of simple mathematical induction, we conclude that $P(n)$ for all natural numbers $n$.
